model/PsacModel.lean
@@ -1,4 +1,5 @@
 import PsacModel.Basic
 import PsacModel.ParLevel
 import PsacModel.Support
+import PsacModel.Scenario
 import PsacModel.Cost
